Minor fixes for verification of Format.*; hints.

src/tls/Format.KeyShareEntry.fst
@@ -8,48 +8,13 @@ module LP = LowParse.SLow
 module U32 = FStar.UInt32
 
 
-(* Types *)
-
-(* 
-   https://tlswg.github.io/tls13-spec/draft-ietf-tls-tls13.html#rfc.section.4.2.8
-
-   struct {
-       NamedGroup group;
-       opaque key_exchange<1..2^16-1>;
-   } KeyShareEntry;
-
-
-   https://tlswg.github.io/tls13-spec/draft-ietf-tls-tls13.html#ffdhe-param
-   
-   Diffie-Hellman [DH] parameters for both clients and servers are encoded in the 
-   opaque key_exchange field of a KeyShareEntry in a KeyShare structure. The opaque
-   value contains the Diffie-Hellman public value (Y = g^X mod p) for the specified
-   group (see [RFC7919] for group definitions) encoded as a big-endian integer
-   and padded to the left with zeros to the size of p in bytes.
-
-
-   https://tlswg.github.io/tls13-spec/draft-ietf-tls-tls13.html#ecdhe-param
-   
-   ECDHE parameters for both clients and servers are encoded in the the opaque 
-   key_exchange field of a KeyShareEntry in a KeyShare structure. 
-   For secp256r1, secp384r1 and secp521r1, the contents are the serialized value
-   of the following struct:
-   
-     struct {
-         uint8 legacy_form = 4;
-         opaque X[coordinate_length];
-         opaque Y[coordinate_length];
-     } UncompressedPointRepresentation;
-
-*)
-
 (* Parsers, validators *)
 
 inline_for_extraction
 let synth_keyShareEntry (r:namedGroup * (LowParse.Spec.Bytes.parse_bounded_vlbytes_t 1 65535)): Tot keyShareEntry = { group=(fst r); key_exchange=(snd r) }
 
 inline_for_extraction
-let unsynth_keyShareEntry (e:keyShareEntry): Tot (namedGroup * B.bytes) = e.group, e.key_exchange
+let unsynth_keyShareEntry (e:keyShareEntry): Tot (namedGroup * (LowParse.Spec.Bytes.parse_bounded_vlbytes_t 1 65535)) = e.group, e.key_exchange
 
 #reset-options "--using_facts_from '* -LowParse -FStar.Reflection -FStar.Tactics'"
 let lemma_synth_keyShareEntry_is_injective () 
@@ -63,9 +28,9 @@ let keyShareEntry_parser_kind' =
 
 let keyShareEntry_parser_kind_metadata = keyShareEntry_parser_kind'.LP.parser_kind_metadata
 
-#reset-options "--using_facts_from '* -LowParse -FStar.Reflection -FStar.Tactics'"
+#reset-options "--using_facts_from '* -FStar.Reflection -FStar.Tactics'"
 
-let keyShareEntry_parser: LP.parser keyShareEntry_parser_kind keyShareEntry =
+let keyShareEntry_parser =
   lemma_synth_keyShareEntry_is_injective ();
   assert_norm (keyShareEntry_parser_kind' == keyShareEntry_parser_kind);
   LP.parse_synth 
@@ -103,18 +68,27 @@ let keyShareEntry_serializer =
     unsynth_keyShareEntry
     ()
 
-let keyShareEntry_serializer32 =
+#reset-options "--using_facts_from '* -LowParse -FStar.Reflection -FStar.Tactics'"
+let keyShareEntry_serializer32: LP.serializer32 keyShareEntry_serializer =
   lemma_synth_keyShareEntry_is_injective ();
   lemma_synth_keyShareEntry_of_unsynth_keyShareEntry ();
   assert_norm (keyShareEntry_parser_kind' == keyShareEntry_parser_kind);
+  lemma_namedGroup_parser_is_strong ();
+  assume (LowParse.SLow.Combinators.serialize32_kind_precond namedGroup_parser_kind (LowParse.Spec.VLData.parse_bounded_vldata_kind 1 65535));
+  assert (LP.synth_inverse synth_keyShareEntry unsynth_keyShareEntry /\ LP.synth_injective synth_keyShareEntry);
+  // cwinter: taramana, what else is missing here (see also Format.Uncompressedpointrepresentation:151 
   LP.serialize32_synth
-    _
+    (namedGroup_parser `LP.nondep_then` (LP.parse_bounded_vlbytes 1 65535))
     synth_keyShareEntry
-    (LP.serialize_nondep_then _ namedGroup_serializer ()
-                              _ (LP.serialize_bounded_vlbytes 1 65535))
-    (LP.serialize32_nondep_then namedGroup_serializer32 ()
-                                (LP.serialize32_bounded_vlbytes 1 65535) ())
+    (LP.serialize_nondep_then 
+      namedGroup_parser namedGroup_serializer ()
+      (LP.parse_bounded_vlbytes 1 65535) (LP.serialize_bounded_vlbytes 1 65535))
+    (LP.serialize32_nondep_then 
+      namedGroup_serializer32 ()
+      (LP.serialize32_bounded_vlbytes 1 65535) ())
     unsynth_keyShareEntry
-    unsynth_keyShareEntry
+    (fun x -> unsynth_keyShareEntry x)
     ()
-   
+#reset-options
+
+
