src/tls/Format.KeyShareEntry.fsti
@@ -6,9 +6,44 @@ module B = FStar.Bytes
 module LP = LowParse.SLow.Base
 module U32 = FStar.UInt32
 
+(* Types *)
+
+(* 
+   https://tlswg.github.io/tls13-spec/draft-ietf-tls-tls13.html#rfc.section.4.2.8
+
+   struct {
+       NamedGroup group;
+       opaque key_exchange<1..2^16-1>;
+   } KeyShareEntry;
+
+
+   https://tlswg.github.io/tls13-spec/draft-ietf-tls-tls13.html#ffdhe-param
+   
+   Diffie-Hellman [DH] parameters for both clients and servers are encoded in the 
+   opaque key_exchange field of a KeyShareEntry in a KeyShare structure. The opaque
+   value contains the Diffie-Hellman public value (Y = g^X mod p) for the specified
+   group (see [RFC7919] for group definitions) encoded as a big-endian integer
+   and padded to the left with zeros to the size of p in bytes.
+
+
+   https://tlswg.github.io/tls13-spec/draft-ietf-tls-tls13.html#ecdhe-param
+   
+   ECDHE parameters for both clients and servers are encoded in the the opaque 
+   key_exchange field of a KeyShareEntry in a KeyShare structure. 
+   For secp256r1, secp384r1 and secp521r1, the contents are the serialized value
+   of the following struct:
+   
+     struct {
+         uint8 legacy_form = 4;
+         opaque X[coordinate_length];
+         opaque Y[coordinate_length];
+     } UncompressedPointRepresentation;
+
+*)
+
 type keyShareEntry = {
   group        : namedGroup; 
-  key_exchange : B.bytes; // (bs:B.bytes{1 <= B.length bs && B.length bs <= 65535});
+  key_exchange : (bs:B.bytes{1 <= B.length bs && B.length bs <= 65535});
 }
 
 inline_for_extraction
