src/tls/Format.UncompressedPointRepresentation.fst
@@ -3,36 +3,40 @@ module Format.UncompressedPointRepresentation
 open Format.Constants
 
 module B = FStar.Bytes
-module U8 = FStar.UInt8
 module U32 = FStar.UInt32
 module LP = LowParse.SLow
 
 unfold type is_injective (#a:Type) (#b:Type) (f:a -> b) 
   = forall x y . f x == f y ==> x == y
-
+ 
 unfold type is_injective_2 (#a:Type) (#b:Type) (f:a -> b) (x:a) (y:a)
   = f x == f y ==> x == y
-
 
 (* Types *)
 
 private 
-type lbytes_pair (coordinate_length:U32.t) = (lbytes32 coordinate_length) * (lbytes32 coordinate_length)
+type lbytes_pair (coordinate_length:coordinate_length_type) 
+  = B.lbytes32 coordinate_length * B.lbytes32 coordinate_length
+  // = (p:(B.lbytes32 coordinate_length * B.lbytes32 coordinate_length)
+  //       {U32.(coordinate_length +^ coordinate_length <^ 512ul) /\
+  //       U32.v coordinate_length + U32.v coordinate_length < 512 /\
+  //       B.length (fst p) + B.length (snd p) < pow2 32 /\
+  //       UInt.fits (B.length (fst p) + B.length (snd p)) 32})
 
 
 (* Parsers *)
 
 private
-let lbytes_pair_parser_kind (coordinate_length:U32.t)
+let lbytes_pair_parser_kind (coordinate_length:coordinate_length_type)
   : LP.parser_kind
   = let l = (UInt32.v coordinate_length) in
     LP.and_then_kind 
       (LP.total_constant_size_parser_kind l)
       (LP.total_constant_size_parser_kind l)
 
-let lbytes_pair_parser (coordinate_length:U32.t)
+let lbytes_pair_parser (coordinate_length:coordinate_length_type)
   : LP.parser (lbytes_pair_parser_kind coordinate_length) (lbytes_pair coordinate_length)
-  = let l = UInt32.v coordinate_length in
+  = let l = U32.v coordinate_length in
     LP.nondep_then
       (LP.parse_flbytes l)
       (LP.parse_flbytes l)
@@ -40,7 +44,7 @@ let lbytes_pair_parser (coordinate_length:U32.t)
 #reset-options "--using_facts_from '* -FStar.Reflection -FStar.Tactics' --max_fuel 16 --initial_fuel 16 --max_ifuel 16 --initial_ifuel 16"
 private
 inline_for_extraction
-let lbytes_pair_parser32 (coordinate_length:U32.t)
+let lbytes_pair_parser32 (coordinate_length:coordinate_length_type)
   : LP.parser32 (lbytes_pair_parser coordinate_length) 
   = let l = UInt32.v coordinate_length in
     LP.parse32_nondep_then
@@ -48,21 +52,21 @@ let lbytes_pair_parser32 (coordinate_length:U32.t)
       (LP.parse32_flbytes l coordinate_length)
 #reset-options
 
-let uncompressedPointRepresentation_parser_kind (coordinate_length:U32.t) 
+let uncompressedPointRepresentation_parser_kind (coordinate_length:coordinate_length_type) 
   = LP.and_then_kind
       constantByte_parser_kind
       (lbytes_pair_parser_kind coordinate_length)
 
 private
 inline_for_extraction
-let ucp_of_uv (#n:U32.t) (p:(lbytes32 n) * (lbytes32 n))
+let ucp_of_uv (#n:coordinate_length_type) (p:(B.lbytes32 n) * (B.lbytes32 n))
   : uncompressedPointRepresentation n
   = { legacy_form = 4uy; x = (fst p); y = (snd p) }
 
 private
 inline_for_extraction
-let uv_of_ucp (#n:U32.t) (x:uncompressedPointRepresentation n)
-  : Tot (lbytes32 n * lbytes32  n)
+let uv_of_ucp (#n:coordinate_length_type) (x:uncompressedPointRepresentation n)
+  : Tot (B.lbytes32 n * B.lbytes32  n)
   = (x.x, x.y)
 
 #reset-options "--using_facts_from '* -LowParse -FStar.Reflection -FStar.Tactics' --max_fuel 16 --initial_fuel 16 --max_ifuel 16 --initial_ifuel 16"
@@ -78,14 +82,14 @@ let lemma_ucp_of_uv_of_ucp #l
 #reset-options
 
 
-let uncompressedPointRepresentation_parser (coordinate_length:U32.t)
+let uncompressedPointRepresentation_parser (coordinate_length:coordinate_length_type)
   : LP.parser (uncompressedPointRepresentation_parser_kind coordinate_length) (uncompressedPointRepresentation coordinate_length) 
   = LP.parse_synth
       (LP.nondep_then (constantByte_parser 4uy) (lbytes_pair_parser coordinate_length))
       (fun (c, uv) -> ucp_of_uv uv)
 
 inline_for_extraction
-let uncompressedPointRepresentation_parser32 (coordinate_length:U32.t)
+let uncompressedPointRepresentation_parser32 (coordinate_length:coordinate_length_type)
   : LP.parser32 (uncompressedPointRepresentation_parser coordinate_length)
   = LP.parse32_synth
       (LP.nondep_then (constantByte_parser 4uy) (lbytes_pair_parser coordinate_length))
@@ -99,7 +103,7 @@ let uncompressedPointRepresentation_parser32 (coordinate_length:U32.t)
 
 #reset-options "--using_facts_from '* -FStar.Reflection -FStar.Tactics' --max_fuel 16 --initial_fuel 16 --max_ifuel 16 --initial_ifuel 16 --z3rlimit 10"
 private
-let lbytes_pair_serializer (coordinate_length:U32.t)
+let lbytes_pair_serializer (coordinate_length:coordinate_length_type)
   : LP.serializer (lbytes_pair_parser coordinate_length) 
   = let l = U32.v coordinate_length in
     let p = LP.parse_flbytes l in
@@ -109,16 +113,16 @@ let lbytes_pair_serializer (coordinate_length:U32.t)
 #reset-options "--using_facts_from '* -FStar.Reflection -FStar.Tactics' --max_fuel 16 --initial_fuel 16 --max_ifuel 16 --initial_ifuel 16 --z3rlimit 10"
 private
 inline_for_extraction
-let lbytes_pair_serializer32 (coordinate_length:U32.t)
+let lbytes_pair_serializer32 (coordinate_length:coordinate_length_type)
   : LP.serializer32 (lbytes_pair_serializer coordinate_length) 
   = let l = U32.v coordinate_length in
     LP.serialize32_nondep_then
       (LP.serialize32_flbytes l) ()
-      (LP.serialize32_flbytes l) (magic ())
+      (LP.serialize32_flbytes l) ()
 #reset-options
 
 
-let uncompressedPointRepresentation_serializer (coordinate_length:U32.t) 
+let uncompressedPointRepresentation_serializer (coordinate_length:coordinate_length_type) 
   : LP.serializer (uncompressedPointRepresentation_parser coordinate_length)
   = lemma_ucp_of_uv_is_injective #coordinate_length;
     lemma_ucp_of_uv_of_ucp #coordinate_length;
@@ -135,21 +139,28 @@ let uncompressedPointRepresentation_serializer (coordinate_length:U32.t)
       (fun ucp -> (ucp.legacy_form, (ucp.x, ucp.y)))
       ()
 
-#reset-options "--using_facts_from '* -FStar.Reflection -FStar.Tactics' --max_fuel 2 --initial_fuel 2 --max_ifuel 2 --initial_ifuel 2 --z3rlimit 10"
+#reset-options "--using_facts_from '* -LowParse -FStar.Reflection -FStar.Tactics' --max_fuel 16 --initial_fuel 16 --max_ifuel 16 --initial_ifuel 16 --z3rlimit 10"
 inline_for_extraction
-let uncompressedPointRepresentation_serializer32 (coordinate_length:U32.t) 
+let uncompressedPointRepresentation_serializer32 (coordinate_length:coordinate_length_type) 
   : LP.serializer32 (uncompressedPointRepresentation_serializer coordinate_length)
   = lemma_ucp_of_uv_is_injective #coordinate_length;
     lemma_ucp_of_uv_of_ucp #coordinate_length;
+    lemma_constantByte_parser_is_strong 4uy;
+    assert (LP.is_strong (constantByte_parser 4uy));
+    assert (constantByte_parser_kind.LP.parser_kind_subkind == Some (LowParse.Spec.Base.ParserStrong));
+    assert (Some? constantByte_parser_kind.LP.parser_kind_high); // cwinter: taramana, why can't it prove the following 2 assertions?
+    assert (Some? (lbytes_pair_parser_kind coordinate_length).LP.parser_kind_high);
+    match constantByte_parser_kind.LP.parser_kind_high, (lbytes_pair_parser_kind coordinate_length).LP.parser_kind_high with 
+    | Some x, Some y -> assert (x + y < 4294967296);
+    assert (LowParse.SLow.Combinators.serialize32_kind_precond constantByte_parser_kind (lbytes_pair_parser_kind coordinate_length));
     LP.serialize32_synth
       _
       (fun (c, uv) -> ucp_of_uv uv)
       _
       (LP.serialize32_nondep_then 
         (constantByte_serializer32 4uy) ()
-        (lbytes_pair_serializer32 coordinate_length) (magic ()))
+        (lbytes_pair_serializer32 coordinate_length) ())
       (fun x -> 4uy, uv_of_ucp x)
       (fun x -> 4uy, uv_of_ucp x)
       ()
 #reset-options
-
