src/tls/Format.NamedGroup.fsti
@@ -4,7 +4,6 @@ module U16 = FStar.UInt16
 module U32 = FStar.UInt32
 module L = FStar.List.Tot
 module LP = LowParse.SLow.Base
-module CC = CoreCrypto
 module B32 = FStar.Bytes
 
 (* Types *)
@@ -79,3 +78,10 @@ val namedGroup_serializer: LP.serializer namedGroup_parser
 
 inline_for_extraction
 val namedGroup_serializer32: LP.serializer32 namedGroup_serializer
+
+
+(* Lemmas *)
+
+val lemma_namedGroup_parser_is_strong (u:unit): 
+  Lemma (LP.is_strong namedGroup_parser /\
+         namedGroup_parser_kind.LP.parser_kind_subkind == Some (LowParse.Spec.Base.ParserStrong))
